template returns isomorphic input

src/equations.v
@@ -72,7 +72,7 @@ Section Template.
                                         is_fine (gen_partition hm [::]) ->
                                         bnodes_of_hash_map hm =i get_bts g -> uniq (relabeling_seq_triple (fun_of_hash_map hm) g).
 
-  Equations? foldl_In {T R : eqType} (s : seq T) (f : R -> forall (y : T), y \in s -> R) (z : R) : R :=
+    Equations? foldl_In {T R : eqType} (s : seq T) (f : R -> forall (y : T), y \in s -> R) (z : R) : R :=
     foldl_In nil f z := z;
     foldl_In (a :: l) f z := foldl_In l (fun x y inP=> f x y _) (f z a _).
   Proof.
@@ -81,7 +81,9 @@ Section Template.
   Qed.
 
   Lemma foldl_foldl_eq {T R : eqType} (s : list T) (f : R -> T -> R) z :
-    @foldl_In _ _ s (fun r t (_ : t \in s) => f r t) z = foldl f z s.
+
+    @foldl_In _ _ s (fun r t (_ : t \in s) => f r t) z =
+      foldl f z s.
   Proof.
     funelim (foldl_In s _ z).
     - by [].
@@ -123,23 +125,24 @@ Section Template.
       distinguish g hm gbot :=
       let p := chose_part hm in
 	    let d := fun bn inP =>
-	                let hm' := color_refine g (mark bn.1 hm) in
-	                if is_fine (gen_partition hm' [::]) then
-	                  let candidate := relabeling_seq_triple (fun_of_hash_map hm') g in
-	                  candidate
-	                else (distinguish g hm' gbot) in
+	    (* let d := fun bn => *)
+	               let hm' := color_refine g (mark bn.1 hm) in
+	               if is_fine (gen_partition hm' [::]) then
+	                 let candidate := relabeling_seq_triple (fun_of_hash_map hm') g in
+	                 candidate
+	               else (distinguish g hm' gbot) in
       let f := fun gbot bn inP  =>
+      (* let f := fun gbot bn  => *)
+                 (* let candidate := d bn in *)
                  let candidate := d bn inP in
                  if cmp gbot candidate then candidate else gbot in
       (* foldl f gbot p. *)
       foldl_In p f gbot.
       Proof.
-      apply /ltP.
-      rewrite nat_coq_nat.
-      eapply (Order.POrderTheory.le_lt_trans). apply color_refineP.
-      rewrite /p in inP.
-      have -> : s = (s,n).1 by [].
-      by apply markP.
+        apply /ltP.
+        rewrite nat_coq_nat.
+        eapply (Order.POrderTheory.le_lt_trans). apply color_refineP.
+        by apply : (markP (s,n)).
       Qed.
 
     Hypothesis init_hash_bnodes : forall (g : seq (triple I B L)), bnodes_of_hash_map (init_hash g) =i get_bts g.
@@ -148,11 +151,13 @@ Section Template.
     Variable can : seq (triple I B L).
     Hypothesis ucan : uniq can.
 
+    Notation le_triple := (@le_triple disp I B L).
+
     Definition template (g : seq (triple I B L)) :=
       let hm := init_hash g in
       let hm' := color g hm in
       let iso_g := if is_fine (gen_partition hm' [::])
-                   then relabeling_seq_triple (fun_of_hash_map hm') g
+                   then (sort le_triple (relabeling_seq_triple (fun_of_hash_map hm') g))
                    else distinguish g hm' can in
       iso_g.
 
@@ -161,7 +166,7 @@ Section Template.
       let f := fun bn =>
 	               let hm' := color_refine g (mark bn.1 hm) in
 	               if is_fine (gen_partition hm' [::]) then
-	                 let candidate := relabeling_seq_triple (fun_of_hash_map hm') g in
+	                 let candidate := sort le_triple (relabeling_seq_triple (fun_of_hash_map hm') g) in
 	                 candidate
 	               else (distinguish g hm' gcan) in
       distinguish g hm gcan = gcan \/ distinguish g hm gcan \in (map f (chose_part hm)).
@@ -177,7 +182,7 @@ Section Template.
       move=> /mapP/= [bn pin ->].
       move=> MH eqbns finePn.
       case : ifP.
-      -  move=> isFine. apply uniq_label_is_fine=> //. apply color_refine_good_hm. apply good_mark. apply eqbns.
+      -  move=> isFine. rewrite sort_uniq. apply uniq_label_is_fine=> //. apply color_refine_good_hm. apply good_mark. apply eqbns.
          by apply in_part_in_bnodes.
       - move=> finePn1. apply IHn.
         eapply Order.POrderTheory.le_lt_trans.
@@ -191,14 +196,93 @@ Section Template.
 
     Lemma uniq_template (g : seq (triple I B L)) (ug: uniq g) : uniq (template g).
     Proof. rewrite /template.
-           case: ifP=> H. by apply fun_of_fine_hash_map_uniq=> //; move=> b; rewrite color_bnodes init_hash_bnodes.
+           case: ifP=> H. rewrite sort_uniq. by apply fun_of_fine_hash_map_uniq=> //; move=> b; rewrite color_bnodes init_hash_bnodes.
            apply uniq_distinguish.
            apply color_good_hm.
            apply good_init.
            by rewrite /= H.
     Qed.
 
-    End Distinguish.
+    Hypothesis piso_sort : forall (g: seq (triple I B L)) (mu : B -> B), is_pre_iso_ts g (sort le_triple (relabeling_seq_triple mu g)) mu <-> is_pre_iso_ts g (relabeling_seq_triple mu g) mu.
+
+    Hypothesis piso_funof : forall (g : seq (triple I B L)) (hm: hash_map),
+        bnodes_hm hm =i get_bts g -> is_fine (gen_partition hm [::]) -> is_pre_iso_ts g (relabeling_seq_triple (fun_of_hash_map hm) g) (fun_of_hash_map hm).
+
+    Hypothesis nil_is_nil : forall g hm, distinguish g hm can = can -> g = can.
+    Hypothesis sort_can : sort le_triple can = can.
+
+    Lemma distinguish_piso : forall (g : seq (triple I B L)) (ug: uniq g), exists mu : B -> B,
+        distinguish g (color g (init_hash g)) can = sort le_triple (relabeling_seq_triple mu g) /\
+          is_pre_iso_ts g (distinguish g (color g (init_hash g)) can) mu.
+    Proof.
+      move=> g ug.
+      set hm := (color g (init_hash g)).
+      have : M hm < S (M hm) by apply ltnSn.
+      have : bnodes_hm hm =i get_bts g by apply color_good_hm; apply good_init.
+      (* rewrite /hm. *)
+      move: hm (M hm).+1.
+      move=> hm n; move: n hm=> n.
+      elim: n => [//| n IHn hm' ghm hmM].
+      (* set hm := (color g (init_hash g)). *)
+      move: (distinguish_choice g hm' can)=> /=[].
+      + move=> H. rewrite H. exists id. split. apply nil_is_nil in H. by rewrite H relabeling_seq_triple_id sort_can.
+        apply nil_is_nil in H.
+        rewrite H.
+        rewrite /is_pre_iso_ts /= /bnode_map_bij.
+        by rewrite (uniq_get_bts _) /= map_id perm_refl.
+      + move=> /mapP/=[bn inp ->].
+        case_eq  (is_fine (gen_partition (color_refine g (mark bn.1 hm')) [::]))=> H.
+        exists (fun_of_hash_map (color_refine g (mark bn.1 hm'))).
+        split=> //.
+        (* rewrite H. *)
+        (* rewrite H. *)
+        apply piso_sort.
+        apply piso_funof.
+        apply color_refine_good_hm. apply good_mark=> //.
+        (* apply color_good_hm. apply good_init. *)
+        by apply in_part_in_bnodes.
+        by apply H.
+      + apply IHn.
+        apply color_refine_good_hm.
+        apply good_mark=> //.
+        by apply in_part_in_bnodes.
+        eapply Order.POrderTheory.le_lt_trans.
+        apply color_refineP.
+        eapply Order.POrderTheory.lt_le_trans.
+        by apply markP.
+        by apply hmM.
+    Qed.
+
+    Lemma preiso_out_template (g : seq (triple I B L)) (ug : uniq g) :
+      exists mu, (template g) = sort le_triple (relabeling_seq_triple mu g) /\ is_pre_iso_ts g (template g) mu.
+    Proof.
+      move/eqP : (eq_refl (template g)).
+      rewrite {2}/template.
+      case: ifP=> is_fine ->.
+      exists (fun_of_hash_map (color g (init_hash g))).
+      split=> //. apply piso_sort. apply piso_funof=> //.
+      apply color_good_hm; apply good_init.
+      by apply distinguish_piso.
+    Qed.
+
+    Hypothesis eiso_sort : forall (g: seq (triple I B L)) (mu : B -> B), effective_iso_ts g (relabeling_seq_triple mu g) ->
+                                                                         effective_iso_ts g (sort le_triple (relabeling_seq_triple mu g)).
+
+    Lemma eiso_out_template (g : seq (triple I B L)) (ug : uniq g) : effective_iso_ts g (template g).
+    Proof.
+      rewrite /iso_ts.
+      move: (uniq_template g ug).
+      suffices [mu  [-> piso utg]]: exists mu, (template g) = sort le_triple (relabeling_seq_triple mu g) /\ is_pre_iso_ts g (template g) mu.
+      rewrite sort_uniq in utg.
+      apply eiso_sort.
+      have {piso}piso : is_pre_iso_ts g (relabeling_seq_triple mu g) mu. apply piso_sort in piso. by apply piso.
+      move : (ts_pre_iso_effective_iso utg piso)=> eiso.
+      by exists mu.
+      by apply preiso_out_template.
+    Qed.
+
+
+  End Distinguish.
 
 
 
